cbor_copy

src/cbor/pulse/raw/CBOR.Pulse.Raw.Copy.fst
@@ -49,7 +49,7 @@ and freeable_cbor_map = {
   map_len: (map_len: SZ.t { SZ.v map_len == V.length map_footprint });
 }
 
-module SM = Pulse.Lib.SeqMatch
+module SM = Pulse.Lib.SeqMatch.Util
 
 let rec freeable_match'
   (x: freeable_cbor')
@@ -74,6 +74,19 @@ and freeable_match_map_entry'
 = freeable_match' c.map_entry_key (fst r) **
   freeable_match' c.map_entry_value (snd r)
 
+let freeable_match_box
+  (bx: freeable_cbor_box)
+  (ft': freeable_tree)
+: Tot slprop
+= exists* (v: cbor_raw) (x': freeable_cbor') . pts_to bx.box_cbor v ** pts_to bx.box_footprint x' ** freeable_match' x' ft'
+
+let freeable_match_box_eq
+  (bx: freeable_cbor_box)
+  (ft': freeable_tree)
+: Lemma
+  (freeable_match' (FBox bx) (FTBox ft') == freeable_match_box bx ft')
+= assert_norm (freeable_match' (FBox bx) (FTBox ft') == freeable_match_box bx ft')
+
 let freeable_match_map_entry
   (c: freeable_cbor_map_entry)
   (r: (freeable_tree & freeable_tree))
@@ -95,6 +108,35 @@ ensures
 {
   unfold (freeable_match_map_entry' r0 freeable_match' c r);
   fold (freeable_match_map_entry c r)
+}
+```
+
+let ftmap_precedes'
+  (r: freeable_tree { FTMap? r })
+: Lemma
+  (FTMap?.m r << r)
+= ()
+
+let ftmap_precedes
+  (r0: list (freeable_tree & freeable_tree))
+: Lemma
+  (ensures (r0 << FTMap r0))
+  [SMTPat (FTMap r0)]
+= ftmap_precedes' (FTMap r0)
+
+```pulse
+ghost
+fn freeable_match_map_entry_weaken_recip
+  (r0: list (freeable_tree & freeable_tree))
+  (c: freeable_cbor_map_entry)
+  (r: (freeable_tree & freeable_tree) { r << r0 })
+requires
+  freeable_match_map_entry c r
+ensures
+  freeable_match_map_entry' (FTMap r0) freeable_match' c r
+{
+  unfold (freeable_match_map_entry c r);
+  fold (freeable_match_map_entry' (FTMap r0) freeable_match' c r);
 }
 ```
 
@@ -254,5 +296,721 @@ ensures
 }
 ```
 
-  
-  
+noeq
+type freeable_cbor = {
+  cbor: cbor_raw;
+  footprint: freeable_cbor';
+  tree: freeable_tree;
+}
+
+let freeable (f: freeable_cbor) : Tot slprop = freeable_match' f.footprint f.tree
+
+```pulse
+fn rec cbor_free
+  (x: freeable_cbor)
+requires
+  freeable x
+ensures
+  emp
+{
+  unfold (freeable x);
+  cbor_free' x.footprint _
+}
+```
+
+open CBOR.Pulse.Raw.Read
+module Trade = Pulse.Lib.Trade.Util
+
+inline_for_extraction
+let cbor_copy_t =
+  (x: cbor_raw) ->
+  (#p: perm) ->
+  (#v: Ghost.erased raw_data_item) ->
+  stt freeable_cbor
+    (cbor_match p x v)
+    (fun res ->
+      cbor_match p x v **
+      cbor_match 1.0R res.cbor v **
+      Trade.trade
+        (cbor_match 1.0R res.cbor v)
+        (freeable res)
+    )
+
+inline_for_extraction
+```pulse
+fn cbor_copy_map_entry
+  (copy: cbor_copy_t)
+  (x: cbor_map_entry)
+  (#p: perm)
+  (#v: Ghost.erased (raw_data_item & raw_data_item))
+requires
+    (cbor_match_map_entry p x v)
+returns res: (freeable_cbor & freeable_cbor)
+ensures
+    (
+      cbor_match_map_entry p x v **
+      cbor_match 1.0R (fst res).cbor (fst v) **
+      cbor_match 1.0R (snd res).cbor (snd v) **
+      Trade.trade
+        (cbor_match 1.0R (fst res).cbor (fst v))
+        (freeable (fst res)) **
+      Trade.trade
+        (cbor_match 1.0R (snd res).cbor (snd v))
+        (freeable (snd res))
+    )
+{
+  unfold (cbor_match_map_entry p x v);
+  let key = copy x.cbor_map_entry_key;
+  let value = copy x.cbor_map_entry_value;
+  fold (cbor_match_map_entry p x v);
+  (key, value)
+}
+```
+
+module S = Pulse.Lib.Slice
+
+inline_for_extraction
+```pulse
+fn rec cbor_copy_array
+  (copy: cbor_copy_t)
+  (x: cbor_raw)
+  (#p: perm)
+  (#v: Ghost.erased raw_data_item)
+requires
+    (cbor_match p x v ** pure (CBOR_Case_Array? x))
+returns res: freeable_cbor
+ensures
+    (
+      cbor_match p x v **
+      cbor_match 1.0R res.cbor v **
+      Trade.trade
+        (cbor_match 1.0R res.cbor v)
+        (freeable res)
+    )
+{
+  cbor_match_cases x;
+  let len64 = cbor_match_array_get_length x;
+  let a = CBOR_Case_Array?.v x;
+  cbor_match_eq_array p a v;
+  Trade.rewrite_with_trade
+    (cbor_match p x v)
+    (cbor_match_array a p v cbor_match);
+  cbor_match_array_elim a p v;
+  Trade.trans _ _ (cbor_match p x v);
+  let ar = a.cbor_array_ptr;
+  S.pts_to_len ar;
+  with ps s pl l . assert (pts_to ar #ps s ** SM.seq_list_match s l (cbor_match pl));
+  SM.seq_list_match_length (cbor_match pl) s l;
+  let len = S.len ar;
+  let v' = V.alloc (CBOR_Case_Simple 0uy (* dummy *)) len;
+  V.pts_to_len v';
+  V.to_array_pts_to v';
+  let ar' = S.from_array (V.vec_to_array v') len;
+  S.pts_to_len ar';
+  let vf = V.alloc FUnit (* dummy *) len;
+  V.pts_to_len vf;
+  with s0 . assert (pts_to ar' s0);
+  with sf0 . assert (pts_to vf sf0);
+  let sl = Ghost.hide (Seq.seq_of_list l);
+  SM.seq_seq_match_empty_intro (cbor_match 1.0R) s0 sl 0;
+  ghost fn aux0 (_: unit)
+  requires emp ** SM.seq_seq_match (cbor_match 1.0R) s0 sl 0 0
+  ensures SM.seq_seq_match freeable_match' sf0 (Seq.create (SZ.v len) FTUnit (* dummy *)) 0 0
+  {
+    SM.seq_seq_match_empty_elim (cbor_match 1.0R) s0 sl 0;
+    SM.seq_seq_match_empty_intro freeable_match' sf0 (Seq.create (SZ.v len) FTUnit (* dummy *)) 0;
+  };
+  Trade.intro _ _ _ aux0;
+  let mut pi = 0sz;
+  while (
+    let i = !pi;
+    (SZ.lt i len)
+  ) invariant b . exists* i s1 j sf st . (
+    pts_to ar #ps s ** SM.seq_list_match s l (cbor_match pl) **
+    pts_to pi i **
+    pts_to ar' s1 **
+    SM.seq_seq_match (cbor_match 1.0R) s1 sl 0 j **
+    pts_to vf sf **
+    Trade.trade
+      (SM.seq_seq_match (cbor_match 1.0R) s1 sl 0 j)
+      (SM.seq_seq_match freeable_match' sf st 0 j) **
+    pure (
+      j == SZ.v i /\
+      j <= SZ.v len /\
+      b == (j < SZ.v len) /\
+      Seq.length st == SZ.v len
+    )
+  ) {
+    S.pts_to_len ar;
+    S.pts_to_len ar';
+    V.pts_to_len vf;
+    let i = !pi;
+    with s1 sf st . assert (pts_to ar' s1 ** pts_to vf sf ** Trade.trade
+      (SM.seq_seq_match (cbor_match 1.0R) s1 sl 0 (SZ.v i))
+      (SM.seq_seq_match freeable_match' sf st 0 (SZ.v i))
+    );
+    let c = S.op_Array_Access ar i;
+    SM.seq_list_match_index_trade (cbor_match pl) s l (SZ.v i);
+    let c' = copy c;
+    Trade.elim _ (SM.seq_list_match s l (cbor_match pl));
+    with v1 . assert (cbor_match 1.0R c'.cbor v1 ** Trade.trade (cbor_match 1.0R c'.cbor v1) (freeable c'));
+    S.op_Array_Assignment ar' i c'.cbor;
+    with s1' . assert (pts_to ar' s1');
+    V.op_Array_Assignment vf i c'.footprint;
+    with sf' . assert (pts_to vf sf');
+    SM.seq_seq_match_rewrite_seq_trade (cbor_match 1.0R) s1 s1' sl sl 0 (SZ.v i);
+    Trade.trans (SM.seq_seq_match (cbor_match 1.0R) s1' sl 0 (SZ.v i)) _ _;
+    Trade.prod (SM.seq_seq_match (cbor_match 1.0R) s1' sl 0 (SZ.v i)) _ (cbor_match 1.0R c'.cbor v1) _;
+    SM.seq_seq_match_enqueue_right_trade (cbor_match 1.0R) s1' sl 0 (SZ.v i) c'.cbor v1;
+    Trade.trans (SM.seq_seq_match (cbor_match 1.0R) s1' sl 0 (SZ.v i + 1)) _ _;
+    let st' = Ghost.hide (Seq.upd st (SZ.v i) c'.tree);
+    ghost fn aux (_: unit)
+    requires emp ** (SM.seq_seq_match freeable_match' sf st 0 (SZ.v i) ** freeable c')
+    ensures SM.seq_seq_match freeable_match' sf' st' 0 (SZ.v i + 1)
+    {
+      SM.seq_seq_match_rewrite_seq freeable_match' sf sf' st st' 0 (SZ.v i);
+      unfold (freeable c');
+      SM.seq_seq_match_enqueue_right freeable_match' sf' st' 0 (SZ.v i) c'.footprint c'.tree;
+    };
+    Trade.intro _ _ _ aux;
+    Trade.trans (SM.seq_seq_match (cbor_match 1.0R) s1' sl 0 (SZ.v i + 1)) _ _;
+    pi := (SZ.add i 1sz);
+  };
+  Trade.elim _ (cbor_match p x v);
+  with s1 sf st . assert (pts_to ar' s1 ** pts_to vf sf ** 
+    SM.seq_seq_match (cbor_match 1.0R) s1 sl 0 (SZ.v len) **
+    Trade.trade
+      (SM.seq_seq_match (cbor_match 1.0R) s1 sl 0 (SZ.v len))
+      (SM.seq_seq_match freeable_match' sf st 0 (SZ.v len))
+  );
+  S.pts_to_len ar';
+  SM.seq_seq_match_seq_list_match_trade (cbor_match 1.0R) s1 sl;
+  Trade.trans _ _ (SM.seq_seq_match freeable_match' sf st 0 (SZ.v len));
+  V.pts_to_len vf;
+  let lt = Ghost.hide (Seq.seq_to_list st);
+  ghost fn auxf (_: unit)
+  requires
+    emp ** SM.seq_seq_match freeable_match' sf st 0 (SZ.v len)
+  ensures SM.seq_list_match sf lt freeable_match'
+  {
+    rewrite (SM.seq_seq_match freeable_match' sf st 0 (SZ.v len))
+      as (SM.seq_seq_match freeable_match' sf (Seq.seq_of_list lt) 0 (SZ.v len));
+    SM.seq_seq_match_seq_list_match freeable_match' sf lt;
+  };
+  Trade.intro _ _ _ auxf;
+  Trade.trans _ _ (SM.seq_list_match sf lt freeable_match');
+  let c' = cbor_match_array_intro len64 ar';
+  Trade.trans_concl_r _ _ _ _;
+  let fa = {
+    array_cbor = v';
+    array_footprint = vf;
+    array_len = len;
+  };
+  let res = {
+    cbor = c';
+    footprint = FArray fa;
+    tree = FTArray lt;
+  };
+  ghost fn aux_res (_: unit)
+  requires
+    (S.is_from_array (V.vec_to_array v') ar' ** pts_to vf sf) **
+    (pts_to ar' s1 ** SM.seq_list_match sf lt freeable_match')
+  ensures
+    freeable res
+  {
+   S.to_array ar';
+   V.to_vec_pts_to v';
+   rewrite (pts_to v' s1) as (pts_to fa.array_cbor s1);
+   rewrite (pts_to vf sf) as (pts_to fa.array_footprint sf);
+   fold (freeable_match' (FArray fa) (FTArray lt));
+   fold (freeable res)
+  };
+  Trade.intro _ _ _ aux_res;
+  Trade.trans _ _ (freeable res);
+  res
+}
+```
+
+#restart-solver
+
+inline_for_extraction
+```pulse
+fn rec cbor_copy_map
+  (copy: cbor_copy_t)
+  (x: cbor_raw)
+  (#p: perm)
+  (#v: Ghost.erased raw_data_item)
+requires
+    (cbor_match p x v ** pure (CBOR_Case_Map? x))
+returns res: freeable_cbor
+ensures
+    (
+      cbor_match p x v **
+      cbor_match 1.0R res.cbor v **
+      Trade.trade
+        (cbor_match 1.0R res.cbor v)
+        (freeable res)
+    )
+{
+  cbor_match_cases x;
+  let len64 = cbor_match_map_get_length x;
+  let a = CBOR_Case_Map?.v x;
+  cbor_match_eq_map0 p a v;
+  Trade.rewrite_with_trade
+    (cbor_match p x v)
+    (cbor_match_map0 a p v cbor_match);
+  cbor_match_map0_map_trade a p v;
+  Trade.trans _ _ (cbor_match p x v);
+  cbor_match_map_elim a p v;
+  Trade.trans _ _ (cbor_match p x v);
+  let ar = a.cbor_map_ptr;
+  S.pts_to_len ar;
+  with ps s pl l . assert (pts_to ar #ps s ** SM.seq_list_match s l (cbor_match_map_entry pl));
+  SM.seq_list_match_length (cbor_match_map_entry pl) s l;
+  let len = S.len ar;
+  let v' = V.alloc
+    ({
+      cbor_map_entry_key = CBOR_Case_Simple 0uy; (* dummy *)
+      cbor_map_entry_value = CBOR_Case_Simple 0uy;
+    })
+    len;
+  V.pts_to_len v';
+  V.to_array_pts_to v';
+  let ar' = S.from_array (V.vec_to_array v') len;
+  S.pts_to_len ar';
+  let vf = V.alloc
+    ({
+      map_entry_key = FUnit;
+      map_entry_value = FUnit;
+    })
+    len;
+  V.pts_to_len vf;
+  with s0 . assert (pts_to ar' s0);
+  with sf0 . assert (pts_to vf sf0);
+  let sl = Ghost.hide (Seq.seq_of_list l);
+  SM.seq_seq_match_empty_intro (cbor_match_map_entry 1.0R) s0 sl 0;
+  ghost fn aux0 (_: unit)
+  requires emp ** SM.seq_seq_match (cbor_match_map_entry 1.0R) s0 sl 0 0
+  ensures SM.seq_seq_match freeable_match_map_entry sf0 (Seq.create (SZ.v len) (FTUnit, FTUnit) (* dummy *)) 0 0
+  {
+    SM.seq_seq_match_empty_elim (cbor_match_map_entry 1.0R) s0 sl 0;
+    SM.seq_seq_match_empty_intro freeable_match_map_entry sf0 (Seq.create (SZ.v len) (FTUnit, FTUnit) (* dummy *)) 0;
+  };
+  Trade.intro _ _ _ aux0;
+  let mut pi = 0sz;
+  while (
+    let i = !pi;
+    (SZ.lt i len)
+  ) invariant b . exists* i s1 j sf st . (
+    pts_to ar #ps s ** SM.seq_list_match s l (cbor_match_map_entry pl) **
+    pts_to pi i **
+    pts_to ar' s1 **
+    SM.seq_seq_match (cbor_match_map_entry 1.0R) s1 sl 0 j **
+    pts_to vf sf **
+    Trade.trade
+      (SM.seq_seq_match (cbor_match_map_entry 1.0R) s1 sl 0 j)
+      (SM.seq_seq_match freeable_match_map_entry sf st 0 j) **
+    pure (
+      j == SZ.v i /\
+      j <= SZ.v len /\
+      b == (j < SZ.v len) /\
+      Seq.length st == SZ.v len
+    )
+  ) {
+    S.pts_to_len ar;
+    S.pts_to_len ar';
+    V.pts_to_len vf;
+    let i = !pi;
+    with s1 sf st . assert (pts_to ar' s1 ** pts_to vf sf ** Trade.trade
+      (SM.seq_seq_match (cbor_match_map_entry 1.0R) s1 sl 0 (SZ.v i))
+      (SM.seq_seq_match freeable_match_map_entry sf st 0 (SZ.v i))
+    );
+    let c = S.op_Array_Access ar i;
+    SM.seq_list_match_index_trade (cbor_match_map_entry pl) s l (SZ.v i);
+    with v1 . assert (cbor_match_map_entry pl c v1);
+    let c' = cbor_copy_map_entry copy c;
+    Trade.elim _ (SM.seq_list_match s l (cbor_match_map_entry pl));
+    Trade.prod
+      (cbor_match 1.0R (fst c').cbor (fst v1))
+      (freeable (fst c'))
+      (cbor_match 1.0R (snd c').cbor (snd v1))
+      (freeable (snd c'));
+    let cme' = {
+      cbor_map_entry_key = (fst c').cbor;
+      cbor_map_entry_value = (snd c').cbor;
+    };
+    Trade.rewrite_with_trade
+      (cbor_match 1.0R (fst c').cbor (fst v1) **
+        cbor_match 1.0R (snd c').cbor (snd v1)
+      )
+      (cbor_match_map_entry 1.0R cme' v1);
+    Trade.trans (cbor_match_map_entry 1.0R cme' v1) _ _;
+    S.op_Array_Assignment ar' i cme';
+    with s1' . assert (pts_to ar' s1');
+    let cfp' = {
+      map_entry_key = (fst c').footprint;
+      map_entry_value = (snd c').footprint;
+    };
+    V.op_Array_Assignment vf i cfp';
+    with sf' . assert (pts_to vf sf');
+    SM.seq_seq_match_rewrite_seq_trade (cbor_match_map_entry 1.0R) s1 s1' sl sl 0 (SZ.v i);
+    Trade.trans (SM.seq_seq_match (cbor_match_map_entry 1.0R) s1' sl 0 (SZ.v i)) _ _;
+    Trade.prod (SM.seq_seq_match (cbor_match_map_entry 1.0R) s1' sl 0 (SZ.v i)) _ (cbor_match_map_entry 1.0R cme' v1) _;
+    SM.seq_seq_match_enqueue_right_trade (cbor_match_map_entry 1.0R) s1' sl 0 (SZ.v i) cme' v1;
+    Trade.trans (SM.seq_seq_match (cbor_match_map_entry 1.0R) s1' sl 0 (SZ.v i + 1)) _ _;
+    let tree = Ghost.hide ((fst c').tree, (snd c').tree);
+    let st' = Ghost.hide (Seq.upd st (SZ.v i) tree);
+    ghost fn aux (_: unit)
+    requires emp ** (SM.seq_seq_match freeable_match_map_entry sf st 0 (SZ.v i) ** (freeable (fst c') ** freeable (snd c')))
+    ensures SM.seq_seq_match freeable_match_map_entry sf' st' 0 (SZ.v i + 1)
+    {
+      SM.seq_seq_match_rewrite_seq freeable_match_map_entry sf sf' st st' 0 (SZ.v i);
+      unfold (freeable (fst c'));
+      unfold (freeable (snd c'));
+      fold (freeable_match_map_entry cfp' tree);
+      SM.seq_seq_match_enqueue_right freeable_match_map_entry sf' st' 0 (SZ.v i) cfp' tree;
+    };
+    Trade.intro _ _ _ aux;
+    Trade.trans (SM.seq_seq_match (cbor_match_map_entry 1.0R) s1' sl 0 (SZ.v i + 1)) _ _;
+    pi := (SZ.add i 1sz);
+  };
+  Trade.elim _ (cbor_match p x v);
+  with s1 sf st . assert (pts_to ar' s1 ** pts_to vf sf ** 
+    SM.seq_seq_match (cbor_match_map_entry 1.0R) s1 sl 0 (SZ.v len) **
+    Trade.trade
+      (SM.seq_seq_match (cbor_match_map_entry 1.0R) s1 sl 0 (SZ.v len))
+      (SM.seq_seq_match freeable_match_map_entry sf st 0 (SZ.v len))
+  );
+  S.pts_to_len ar';
+  SM.seq_seq_match_seq_list_match_trade (cbor_match_map_entry 1.0R) s1 sl;
+  Trade.trans _ _ (SM.seq_seq_match freeable_match_map_entry sf st 0 (SZ.v len));
+  V.pts_to_len vf;
+  let lt = Ghost.hide (Seq.seq_to_list st);
+  ghost fn auxf (_: unit)
+  requires
+    emp ** SM.seq_seq_match freeable_match_map_entry sf st 0 (SZ.v len)
+  ensures SM.seq_list_match sf lt (freeable_match_map_entry' (FTMap lt) freeable_match')
+  {
+    rewrite (SM.seq_seq_match freeable_match_map_entry sf st 0 (SZ.v len))
+      as (SM.seq_seq_match freeable_match_map_entry sf (Seq.seq_of_list lt) 0 (SZ.v len));
+    SM.seq_seq_match_seq_list_match freeable_match_map_entry sf lt;
+    SM.seq_list_match_weaken sf lt freeable_match_map_entry (freeable_match_map_entry' (FTMap lt) freeable_match') (freeable_match_map_entry_weaken_recip lt);
+  };
+  Trade.intro _ _ _ auxf;
+  Trade.trans _ _ (SM.seq_list_match sf lt (freeable_match_map_entry' (FTMap lt) freeable_match'));
+  let c' = cbor_match_map_intro len64 ar';
+  Trade.trans_concl_r _ _ _ _;
+  let fa = {
+    map_cbor = v';
+    map_footprint = vf;
+    map_len = len;
+  };
+  let res = {
+    cbor = c';
+    footprint = FMap fa;
+    tree = FTMap lt;
+  };
+  ghost fn aux_res (_: unit)
+  requires
+    (S.is_from_array (V.vec_to_array v') ar' ** pts_to vf sf) **
+    (pts_to ar' s1 ** SM.seq_list_match sf lt (freeable_match_map_entry' (FTMap lt) freeable_match'))
+  ensures
+    freeable res
+  {
+   S.to_array ar';
+   V.to_vec_pts_to v';
+   rewrite (pts_to v' s1) as (pts_to fa.map_cbor s1);
+   rewrite (pts_to vf sf) as (pts_to fa.map_footprint sf);
+   fold (freeable_match' (FMap fa) (FTMap lt));
+   fold (freeable res)
+  };
+  Trade.intro _ _ _ aux_res;
+  Trade.trans _ _ (freeable res);
+  res
+}
+```
+
+```pulse
+fn rec cbor_copy
+  (x: cbor_raw)
+  (#p: perm)
+  (#v: Ghost.erased raw_data_item)
+requires
+    (cbor_match p x v)
+returns res: freeable_cbor
+ensures
+    (
+      cbor_match p x v **
+      cbor_match 1.0R res.cbor v **
+      Trade.trade
+        (cbor_match 1.0R res.cbor v)
+        (freeable res)
+    )
+{
+  cbor_match_cases x;
+  match x {
+    CBOR_Case_Int _ -> {
+      let ty = cbor_match_int_elim_type x;
+      let w = cbor_match_int_elim_value x;
+      let c' = cbor_match_int_intro ty w;
+      let res = {
+        cbor = c';
+        footprint = FUnit;
+        tree = FTUnit;
+      };
+      ghost fn aux (_: unit)
+      requires emp ** cbor_match 1.0R c' (Int64 ty w)
+      ensures freeable res
+      {
+        cbor_match_int_free c';
+        fold (freeable_match' FUnit FTUnit);
+        fold (freeable res)
+      };
+      Trade.intro_trade _ _ _ aux;
+      res
+    }
+    CBOR_Case_Simple _ -> {
+      let w = cbor_match_simple_elim x;
+      let c' = cbor_match_simple_intro w;
+      let res = {
+        cbor = c';
+        footprint = FUnit;
+        tree = FTUnit;
+      };
+      ghost fn aux (_: unit)
+      requires emp ** cbor_match 1.0R c' (Simple w)
+      ensures freeable res
+      {
+        cbor_match_simple_free c';
+        fold (freeable_match' FUnit FTUnit);
+        fold (freeable res)
+      };
+      Trade.intro_trade _ _ _ aux;
+      res
+    }
+    CBOR_Case_String _ -> {
+      let ty = cbor_match_string_elim_type x;
+      let len = cbor_match_string_elim_length x;
+      let pl = cbor_match_string_elim_payload x;
+      S.pts_to_len pl;
+      let len_sz = S.len pl;
+      let v' = V.alloc 0uy len_sz;
+      V.to_array_pts_to v';
+      let s' = S.from_array (V.vec_to_array v') len_sz;
+      S.pts_to_len s';
+      S.copy s' pl;
+      Trade.elim _ _;
+      with vs' . assert (pts_to s' vs');
+      let c' = cbor_match_string_intro ty len s';
+      let res = {
+        cbor = c';
+        footprint = FBytes v';
+        tree = FTBytes;
+      };
+      ghost fn aux (_: unit)
+      requires S.is_from_array (V.vec_to_array v') s' ** pts_to s' vs'
+      ensures freeable res
+      {
+        S.to_array s';
+        V.to_vec_pts_to v';
+        fold (freeable_match' (FBytes v') FTBytes);
+        fold (freeable res)
+      };
+      Trade.intro _ _ _ aux;
+      Trade.trans _ (pts_to s' vs') _;
+      res
+    }
+    CBOR_Case_Tagged _ -> {
+      let tag = cbor_match_tagged_get_tag x;
+      let pl = cbor_match_tagged_get_payload x;
+      let cpl' = cbor_copy pl;
+      Trade.elim _ (cbor_match p x v);
+      let bf = B.alloc cpl'.footprint;
+      let b = B.alloc cpl'.cbor;
+      B.to_ref_pts_to b;
+      let c' = cbor_match_tagged_intro tag (B.box_to_ref b);
+      Trade.trans_concl_r _ _ _ _;
+      let fb = {
+          box_cbor = b;
+          box_footprint = bf;
+      };
+      let res = {
+        cbor = c';
+        footprint = FBox fb;
+        tree = FTBox cpl'.tree
+      };
+      ghost fn aux (_: unit)
+      requires
+        (pts_to bf cpl'.footprint ** (pts_to (B.box_to_ref b) cpl'.cbor ** freeable cpl'))
+      ensures
+        (freeable res)
+      {
+        B.to_box_pts_to b;
+        rewrite (pts_to bf cpl'.footprint) as (pts_to fb.box_footprint cpl'.footprint);
+        rewrite (pts_to b cpl'.cbor) as (pts_to fb.box_cbor) (cpl'.cbor);
+        unfold (freeable cpl');
+        fold (freeable_match_box fb cpl'.tree);
+        freeable_match_box_eq fb cpl'.tree;
+        rewrite (freeable_match_box fb cpl'.tree) as (freeable_match' (FBox fb) (FTBox cpl'.tree));
+        fold (freeable res)
+      };
+      Trade.intro _ _ _ aux;
+      Trade.trans _ _ (freeable res);
+      res
+    }
+    CBOR_Case_Array a -> {
+      cbor_copy_array cbor_copy (CBOR_Case_Array a);
+    }
+    CBOR_Case_Map a -> {
+      cbor_copy_map cbor_copy (CBOR_Case_Map a);
+    }
+    CBOR_Case_Serialized_Array a -> {
+      Trade.rewrite_with_trade
+        (cbor_match p x v)
+        (cbor_match_serialized_array a p v);
+      unfold (cbor_match_serialized_array a p v);
+      let len = S.len a.cbor_serialized_payload;
+      let v' = V.alloc 0uy len;
+      V.pts_to_len v';
+      V.to_array_pts_to v';
+      let s' = S.from_array (V.vec_to_array v') len;
+      S.pts_to_len s';
+      cbor_match_serialized_payload_array_copy a.cbor_serialized_payload _ _ s';
+      fold (cbor_match_serialized_array a p v);
+      Trade.elim _ (cbor_match p x v);
+      let a' = {
+        cbor_serialized_header = a.cbor_serialized_header;
+        cbor_serialized_payload = s';
+        cbor_serialized_perm = 1.0R;
+      };
+      fold (cbor_match_serialized_array a' 1.0R v);
+      let res = {
+        cbor = CBOR_Case_Serialized_Array a';
+        footprint = FBytes v';
+        tree = FTBytes;
+      };
+      ghost fn aux (_: unit)
+      requires
+        (
+          Trade.trade
+            (cbor_match_serialized_payload_array s' 1.0R (Array?.v v))
+            (exists* v_ . pts_to s' v_) **
+          S.is_from_array (V.vec_to_array v') s'
+        ) ** cbor_match_serialized_array a' 1.0R v
+      ensures freeable res
+      {
+        unfold (cbor_match_serialized_array a' 1.0R v);
+        Trade.elim _ _;
+        S.to_array s';
+        V.to_vec_pts_to v';
+        fold (freeable_match' (FBytes v') FTBytes);
+        fold (freeable res)
+      };
+      Trade.intro _ _ _ aux;
+      Trade.rewrite_with_trade
+        (cbor_match_serialized_array a' 1.0R v)
+        (cbor_match 1.0R res.cbor v);
+      Trade.trans (cbor_match 1.0R res.cbor v) _ _;
+      res
+    }
+    CBOR_Case_Serialized_Map a -> {
+      Trade.rewrite_with_trade
+        (cbor_match p x v)
+        (cbor_match_serialized_map a p v);
+      unfold (cbor_match_serialized_map a p v);
+      let len = S.len a.cbor_serialized_payload;
+      let v' = V.alloc 0uy len;
+      V.pts_to_len v';
+      V.to_array_pts_to v';
+      let s' = S.from_array (V.vec_to_array v') len;
+      S.pts_to_len s';
+      cbor_match_serialized_payload_map_copy a.cbor_serialized_payload _ _ s';
+      fold (cbor_match_serialized_map a p v);
+      Trade.elim _ (cbor_match p x v);
+      let a' = {
+        cbor_serialized_header = a.cbor_serialized_header;
+        cbor_serialized_payload = s';
+        cbor_serialized_perm = 1.0R;
+      };
+      fold (cbor_match_serialized_map a' 1.0R v);
+      let res = {
+        cbor = CBOR_Case_Serialized_Map a';
+        footprint = FBytes v';
+        tree = FTBytes;
+      };
+      ghost fn aux (_: unit)
+      requires
+        (
+          Trade.trade
+            (cbor_match_serialized_payload_map s' 1.0R (Map?.v v))
+            (exists* v_ . pts_to s' v_) **
+          S.is_from_array (V.vec_to_array v') s'
+        ) ** cbor_match_serialized_map a' 1.0R v
+      ensures freeable res
+      {
+        unfold (cbor_match_serialized_map a' 1.0R v);
+        Trade.elim _ _;
+        S.to_array s';
+        V.to_vec_pts_to v';
+        fold (freeable_match' (FBytes v') FTBytes);
+        fold (freeable res)
+      };
+      Trade.intro _ _ _ aux;
+      Trade.rewrite_with_trade
+        (cbor_match_serialized_map a' 1.0R v)
+        (cbor_match 1.0R res.cbor v);
+      Trade.trans (cbor_match 1.0R res.cbor v) _ _;
+      res
+    }
+    CBOR_Case_Serialized_Tagged a -> {
+      Trade.rewrite_with_trade
+        (cbor_match p x v)
+        (cbor_match_serialized_tagged a p v);
+      unfold (cbor_match_serialized_tagged a p v);
+      let len = S.len a.cbor_serialized_payload;
+      let v' = V.alloc 0uy len;
+      V.pts_to_len v';
+      V.to_array_pts_to v';
+      let s' = S.from_array (V.vec_to_array v') len;
+      S.pts_to_len s';
+      cbor_match_serialized_payload_tagged_copy a.cbor_serialized_payload _ _ s';
+      fold (cbor_match_serialized_tagged a p v);
+      Trade.elim _ (cbor_match p x v);
+      let a' = {
+        cbor_serialized_header = a.cbor_serialized_header;
+        cbor_serialized_payload = s';
+        cbor_serialized_perm = 1.0R;
+      };
+      fold (cbor_match_serialized_tagged a' 1.0R v);
+      let res = {
+        cbor = CBOR_Case_Serialized_Tagged a';
+        footprint = FBytes v';
+        tree = FTBytes;
+      };
+      ghost fn aux (_: unit)
+      requires
+        (
+          Trade.trade
+            (cbor_match_serialized_payload_tagged s' 1.0R (Tagged?.v v))
+            (exists* v_ . pts_to s' v_) **
+          S.is_from_array (V.vec_to_array v') s'
+        ) ** cbor_match_serialized_tagged a' 1.0R v
+      ensures freeable res
+      {
+        unfold (cbor_match_serialized_tagged a' 1.0R v);
+        Trade.elim _ _;
+        S.to_array s';
+        V.to_vec_pts_to v';
+        fold (freeable_match' (FBytes v') FTBytes);
+        fold (freeable res)
+      };
+      Trade.intro _ _ _ aux;
+      Trade.rewrite_with_trade
+        (cbor_match_serialized_tagged a' 1.0R v)
+        (cbor_match 1.0R res.cbor v);
+      Trade.trans (cbor_match 1.0R res.cbor v) _ _;
+      res
+    }
+  }
+}
+```
