src/cbor/pulse/raw/everparse/CBOR.Pulse.Raw.Format.Match.fst
@@ -20,3 +20,128 @@ let cbor_match_serialized_payload_map
 let cbor_match_serialized_payload_tagged
   c p r
 = pts_to_serialized serialize_raw_data_item c #p r
+
+#set-options "--print_implicits"
+
+```pulse
+fn cbor_match_serialized_payload_array_copy
+  (c: slice U8.t)
+  (p: perm)
+  (r: Ghost.erased (list raw_data_item))
+  (c': slice U8.t)
+requires
+    (exists* v' . pts_to c' v' **
+      cbor_match_serialized_payload_array c p r **
+      pure (len c == len c')
+    )
+ensures
+    (
+      cbor_match_serialized_payload_array c p r **
+      cbor_match_serialized_payload_array c' 1.0R r **
+      Trade.trade
+        (cbor_match_serialized_payload_array c' 1.0R r)
+        (exists* v' . pts_to c' v')
+    )
+{
+  unfold (cbor_match_serialized_payload_array c p r);
+  with n r' . assert (
+    pts_to_serialized (serialize_nlist n serialize_raw_data_item) c #p r'
+  );
+  pts_to_serialized_copy #(nlist n raw_data_item) #(parse_nlist_kind n parse_raw_data_item_kind) #(coerce_eq () (parse_nlist n parse_raw_data_item)) (coerce_eq () (serialize_nlist n serialize_raw_data_item <: serializer (parse_nlist n parse_raw_data_item))) c c';
+  fold (cbor_match_serialized_payload_array c p r);
+  fold (cbor_match_serialized_payload_array c' 1.0R r);
+  ghost fn aux (_: unit)
+  requires emp ** cbor_match_serialized_payload_array c' 1.0R r
+  ensures exists* v' . pts_to c' v'
+  {
+    unfold (cbor_match_serialized_payload_array c' 1.0R r);
+    with n r' . assert (
+      pts_to_serialized (serialize_nlist n serialize_raw_data_item) c' r'
+    );
+    unfold (pts_to_serialized (serialize_nlist n serialize_raw_data_item) c' r')
+  };
+  Trade.intro_trade _ _ _ aux
+}
+```
+
+```pulse
+fn cbor_match_serialized_payload_map_copy
+  (c: slice U8.t)
+  (p: perm)
+  (r: Ghost.erased (list (raw_data_item & raw_data_item)))
+  (c': slice U8.t)
+requires
+    (exists* v' . pts_to c' v' **
+      cbor_match_serialized_payload_map c p r **
+      pure (len c == len c')
+    )
+ensures
+    (
+      cbor_match_serialized_payload_map c p r **
+      cbor_match_serialized_payload_map c' 1.0R r **
+      Trade.trade
+        (cbor_match_serialized_payload_map c' 1.0R r)
+        (exists* v' . pts_to c' v')
+    )
+{
+  unfold (cbor_match_serialized_payload_map c p r);
+  with n r' . assert (
+    pts_to_serialized (serialize_nlist n (serialize_nondep_then serialize_raw_data_item serialize_raw_data_item)) c #p r'
+  );
+  pts_to_serialized_copy #(nlist n (raw_data_item & raw_data_item)) #(parse_nlist_kind n (and_then_kind parse_raw_data_item_kind parse_raw_data_item_kind)) #(coerce_eq () (parse_nlist n (nondep_then parse_raw_data_item parse_raw_data_item))) (coerce_eq () (serialize_nlist n (serialize_nondep_then serialize_raw_data_item serialize_raw_data_item) <: serializer (parse_nlist n (nondep_then parse_raw_data_item parse_raw_data_item)))) c c';
+  fold (cbor_match_serialized_payload_map c p r);
+  fold (cbor_match_serialized_payload_map c' 1.0R r);
+  ghost fn aux (_: unit)
+  requires emp ** cbor_match_serialized_payload_map c' 1.0R r
+  ensures exists* v' . pts_to c' v'
+  {
+    unfold (cbor_match_serialized_payload_map c' 1.0R r);
+    with n r' . assert (
+      pts_to_serialized (serialize_nlist n (serialize_nondep_then serialize_raw_data_item serialize_raw_data_item)) c' r'
+    );
+    unfold (pts_to_serialized (serialize_nlist n (serialize_nondep_then serialize_raw_data_item serialize_raw_data_item)) c' r')
+  };
+  Trade.intro_trade _ _ _ aux
+}
+```
+
+```pulse
+fn cbor_match_serialized_payload_tagged_copy
+  (c: slice U8.t)
+  (p: perm)
+  (r: Ghost.erased (raw_data_item))
+  (c': slice U8.t)
+requires
+    (exists* v' . pts_to c' v' **
+      cbor_match_serialized_payload_tagged c p r **
+      pure (len c == len c')
+    )
+ensures
+    (
+      cbor_match_serialized_payload_tagged c p r **
+      cbor_match_serialized_payload_tagged c' 1.0R r **
+      Trade.trade
+        (cbor_match_serialized_payload_tagged c' 1.0R r)
+        (exists* v' . pts_to c' v')
+    )
+{
+  unfold (cbor_match_serialized_payload_tagged c p r);
+  with r' . assert (
+    pts_to_serialized (serialize_raw_data_item) c #p r'
+  );
+  pts_to_serialized_copy serialize_raw_data_item c c';
+  fold (cbor_match_serialized_payload_tagged c p r);
+  fold (cbor_match_serialized_payload_tagged c' 1.0R r);
+  ghost fn aux (_: unit)
+  requires emp ** cbor_match_serialized_payload_tagged c' 1.0R r
+  ensures exists* v' . pts_to c' v'
+  {
+    unfold (cbor_match_serialized_payload_tagged c' 1.0R r);
+    with r' . assert (
+      pts_to_serialized (serialize_raw_data_item) c' r'
+    );
+    unfold (pts_to_serialized (serialize_raw_data_item) c' r')
+  };
+  Trade.intro_trade _ _ _ aux
+}
+```
