src/cbor/pulse/raw/CBOR.Pulse.Raw.Format.Match.fsti
@@ -6,6 +6,7 @@ open Pulse.Lib.Slice
 
 module U8 = FStar.UInt8
 module SZ = FStar.SizeT
+module Trade = Pulse.Lib.Trade
 
 val cbor_match_serialized_payload_array
   (c: slice U8.t)
@@ -24,3 +25,57 @@ val cbor_match_serialized_payload_tagged
   (p: perm)
   (r: raw_data_item)
 : Tot slprop
+
+val cbor_match_serialized_payload_array_copy
+  (c: slice U8.t)
+  (p: perm)
+  (r: Ghost.erased (list raw_data_item))
+  (c': slice U8.t)
+: stt unit
+    (exists* v' . pts_to c' v' **
+      cbor_match_serialized_payload_array c p r **
+      pure (len c == len c')
+    )
+    (fun _ ->
+      cbor_match_serialized_payload_array c p r **
+      cbor_match_serialized_payload_array c' 1.0R r **
+      Trade.trade
+        (cbor_match_serialized_payload_array c' 1.0R r)
+        (exists* v' . pts_to c' v')
+    )
+
+val cbor_match_serialized_payload_map_copy
+  (c: slice U8.t)
+  (p: perm)
+  (r: Ghost.erased (list (raw_data_item & raw_data_item)))
+  (c': slice U8.t)
+: stt unit
+    (exists* v' . pts_to c' v' **
+      cbor_match_serialized_payload_map c p r **
+      pure (len c == len c')
+    )
+    (fun _ ->
+      cbor_match_serialized_payload_map c p r **
+      cbor_match_serialized_payload_map c' 1.0R r **
+      Trade.trade
+        (cbor_match_serialized_payload_map c' 1.0R r)
+        (exists* v' . pts_to c' v')
+    )
+
+val cbor_match_serialized_payload_tagged_copy
+  (c: slice U8.t)
+  (p: perm)
+  (r: Ghost.erased raw_data_item)
+  (c': slice U8.t)
+: stt unit
+    (exists* v' . pts_to c' v' **
+      cbor_match_serialized_payload_tagged c p r **
+      pure (len c == len c')
+    )
+    (fun _ ->
+      cbor_match_serialized_payload_tagged c p r **
+      cbor_match_serialized_payload_tagged c' 1.0R r **
+      Trade.trade
+        (cbor_match_serialized_payload_tagged c' 1.0R r)
+        (exists* v' . pts_to c' v')
+    )
